pulse/lib/pulse/core/PulseCore.Action.fsti
@@ -27,15 +27,14 @@ open PulseCore.InstantiatedSemantics
 
 type reifiability =
  | Ghost
- | Reifiable
+ | Atomic
 
 let ( ^^ ) (r1 r2 : reifiability) : reifiability =
   if r1 = r2 then r1
-  else Reifiable
+  else Atomic
 
 [@@ erasable]
 val iref : Type0
-val storable_iref (i:iref) : GTot bool
 val deq_iref : FStar.GhostSet.decide_eq iref
 let inames = FStar.GhostSet.set iref
 let singleton (i:iref) : inames = GhostSet.singleton deq_iref i
@@ -86,13 +85,13 @@ val frame
      (f:act a r opens pre post)
 : act a r opens (pre ** frame) (fun x -> post x ** frame)
 
-val lift_ghost_reifiable
+val lift_ghost_atomic
     (#a:Type)
     (#pre:slprop)
     (#post:a -> slprop)
     (#opens:inames)
     (f:act a Ghost opens pre post)
-: act a Reifiable opens pre post
+: act a Atomic opens pre post
 
 val weaken 
     (#a:Type)
@@ -142,30 +141,19 @@ let add_inv (e:inames) (i:iref) : inames = GhostSet.union (singleton i) e
 let mem_inv (e:inames) (i:iref) : GTot bool = GhostSet.mem i e
 
 val inv (i:iref) (p:slprop) : slprop
-val storable_inv (i:iref { storable_iref i }) (p:slprop3)
-: Lemma (is_slprop3 (inv i p))
-let live (i:iref) = exists* (p:slprop). inv i p
-
-let rec all_live (ctx:list iref) =
-  match ctx with
-  | [] -> emp
-  | hd::tl -> live hd ** all_live tl
 
 val dup_inv (i:iref) (p:slprop)
   : act unit Ghost emp_inames (inv i p) (fun _ -> (inv i p) ** (inv i p))
 
-val new_invariant (p:slprop3)
+val new_invariant (p:slprop)
 : act iref Ghost emp_inames p (fun i -> inv i p)
-
-val new_storable_invariant (p:slprop2)
-: act (i:iref{storable_iref i}) Ghost emp_inames p (fun i -> inv i p)
 
 let fresh_wrt (i:iref)
               (ctx:list iref)
 : prop
 = forall i'. List.Tot.memP i' ctx ==> i' =!= i
 
-val fresh_invariant (ctx:list iref) (p:slprop3)
+val fresh_invariant (ctx:list iref) (p:slprop)
 : act (i:iref { i `fresh_wrt` ctx }) Ghost emp_inames p (fun i -> inv i p)
 
 val with_invariant
@@ -176,19 +164,19 @@ val with_invariant
     (#f_opens:inames)
     (#p:slprop)
     (i:iref { not (mem_inv f_opens i) })
-    (f:unit -> act a r f_opens (p ** fp) (fun x -> p ** fp' x))
+    (f:unit -> act a r f_opens (later p ** fp) (fun x -> later p ** fp' x))
 : act a r (add_inv f_opens i) ((inv i p) ** fp) (fun x -> (inv i p) ** fp' x)
 
-val distinct_invariants_have_distinct_names
-    (#p:slprop)
-    (#q:slprop)
-    (i j:iref)
-    (_:squash (p =!= q))
-: act (squash (i =!= j))
-      Ghost
-      emp_inames 
-      ((inv i p) ** (inv j q))
-      (fun _ -> (inv i p) ** (inv j q))
+// val distinct_invariants_have_distinct_names
+//     (#p:slprop)
+//     (#q:slprop)
+//     (i j:iref)
+//     (_:squash (p =!= q))
+// : act (squash (i =!= j))
+//       Ghost
+//       emp_inames 
+//       ((inv i p) ** (inv j q))
+//       (fun _ -> (inv i p) ** (inv j q))
 
 val invariant_name_identifies_invariant
       (p q:slprop)
@@ -197,8 +185,8 @@ val invariant_name_identifies_invariant
 : act (squash (p == q))
       Ghost
       emp_inames
-      ((inv i p) ** (inv j q))
-      (fun _ -> (inv i p) ** (inv j q))
+      (inv i p ** inv j q)
+      (fun _ -> inv i p ** inv j q ** equiv p q)
 
 
 ////////////////////////////////////////////////////////////////////////
@@ -215,7 +203,7 @@ let is_ref_null (#a:Type) (#p:FStar.PCM.pcm a) (r:ref a p)
 : b:bool { b <==> r == ref_null p }
 = is_core_ref_null r
 
-val pts_to (#a:Type u#1) (#p:pcm a) (r:ref a p) (v:a) : slprop2
+val pts_to (#a:Type u#1) (#p:pcm a) (r:ref a p) (v:a) : slprop
 
 val pts_to_not_null (#a:Type) (#p:FStar.PCM.pcm a) (r:ref a p) (v:a)
 : act (squash (not (is_ref_null r)))
@@ -229,7 +217,7 @@ val alloc
     (#pcm:pcm a)
     (x:a{pcm.refine x})
 : act (ref a pcm)
-      Reifiable
+      Atomic
       emp_inames
       emp
       (fun r -> pts_to r x)
@@ -243,7 +231,7 @@ val read
         -> GTot (y:a{compatible p y v /\
                      FStar.PCM.frame_compatible p x v y})))
 : act (v:a{compatible p x v /\ p.refine v})
-      Reifiable
+      Atomic
       emp_inames
       (pts_to r x)
       (fun v -> pts_to r (f v))
@@ -255,7 +243,7 @@ val write
     (x y:Ghost.erased a)
     (f:FStar.PCM.frame_preserving_upd p x y)
 : act unit
-    Reifiable
+    Atomic
     emp_inames
     (pts_to r x)
     (fun _ -> pts_to r y)
@@ -288,7 +276,7 @@ val gather
 // Big references
 ///////////////////////////////////////////////////////////////////
 
-val big_pts_to (#a:Type u#2) (#p:pcm a) (r:ref a p) (v:a) : slprop3
+val big_pts_to (#a:Type u#2) (#p:pcm a) (r:ref a p) (v:a) : slprop
 
 val big_pts_to_not_null (#a:Type) (#p:FStar.PCM.pcm a) (r:ref a p) (v:a)
 : act (squash (not (is_ref_null r)))
@@ -302,7 +290,7 @@ val big_alloc
     (#pcm:pcm a)
     (x:a{pcm.refine x})
 : act (ref a pcm)
-      Reifiable
+      Atomic
       emp_inames
       emp
       (fun r -> big_pts_to r x)
@@ -316,7 +304,7 @@ val big_read
         -> GTot (y:a{compatible p y v /\
                      FStar.PCM.frame_compatible p x v y})))
 : act (v:a{compatible p x v /\ p.refine v})
-      Reifiable
+      Atomic
       emp_inames
       (big_pts_to r x)
       (fun v -> big_pts_to r (f v))
@@ -328,7 +316,7 @@ val big_write
     (x y:Ghost.erased a)
     (f:FStar.PCM.frame_preserving_upd p x y)
 : act unit
-    Reifiable
+    Atomic
     emp_inames
     (big_pts_to r x)
     (fun _ -> big_pts_to r y)
@@ -375,7 +363,7 @@ val nb_alloc
     (#pcm:pcm a)
     (x:a{pcm.refine x})
 : act (ref a pcm)
-      Reifiable
+      Atomic
       emp_inames
       emp
       (fun r -> nb_pts_to r x)
@@ -389,7 +377,7 @@ val nb_read
         -> GTot (y:a{compatible p y v /\
                      FStar.PCM.frame_compatible p x v y})))
 : act (v:a{compatible p x v /\ p.refine v})
-      Reifiable
+      Atomic
       emp_inames
       (nb_pts_to r x)
       (fun v -> nb_pts_to r (f v))
@@ -401,7 +389,7 @@ val nb_write
     (x y:Ghost.erased a)
     (f:FStar.PCM.frame_preserving_upd p x y)
 : act unit
-    Reifiable
+    Atomic
     emp_inames
     (nb_pts_to r x)
     (fun _ -> nb_pts_to r y)
@@ -463,7 +451,7 @@ val drop (p:slprop)
 [@@erasable]
 val core_ghost_ref : Type u#0
 let ghost_ref (#a:Type u#a) (p:pcm a) : Type u#0 = core_ghost_ref
-val ghost_pts_to (#a:Type u#1) (#p:pcm a) (r:ghost_ref p) (v:a) : slprop2
+val ghost_pts_to (#a:Type u#1) (#p:pcm a) (r:ghost_ref p) (v:a) : slprop
 
 val ghost_alloc
     (#a:Type u#1)
@@ -515,7 +503,7 @@ val ghost_gather
     (ghost_pts_to r v0 ** ghost_pts_to r v1)
     (fun _ -> ghost_pts_to r (op pcm v0 v1))
 
-val big_ghost_pts_to (#a:Type u#2) (#p:pcm a) (r:ghost_ref p) (v:a) : slprop3
+val big_ghost_pts_to (#a:Type u#2) (#p:pcm a) (r:ghost_ref p) (v:a) : slprop
 
 val big_ghost_alloc
     (#a:Type)
