pulse/lib/pulse/core/PulseCore.Atomic.fsti
@@ -250,13 +250,10 @@ val ghost_reveal (a:Type) (x:erased a)
 val dup_inv (i:iref) (p:slprop)
   : stt_ghost unit emp_inames (inv i p) (fun _ -> (inv i p) ** (inv i p))
 
-val new_invariant (p:slprop3)
+val new_invariant (p:slprop)
   : stt_ghost iref emp_inames p (fun i -> inv i p)
 
-val new_storable_invariant (p:slprop2)
-  : stt_ghost (i:iref { storable_iref i }) emp_inames p (fun i -> inv i p)
-
-val fresh_invariant (ctx:list iref) (p:slprop3)
+val fresh_invariant (ctx:list iref) (p:slprop)
 : stt_ghost (i:iref { i `fresh_wrt` ctx })
             emp_inames
             p
@@ -271,8 +268,8 @@ val with_invariant
     (#p:slprop)
     (i:iref { not (mem_inv f_opens i) })
     ($f:unit -> stt_atomic a #obs f_opens
-                           (p ** fp)
-                           (fun x -> p ** fp' x))
+                           (later p ** fp)
+                           (fun x -> later p ** fp' x))
 : stt_atomic a #obs (add_inv f_opens i) ((inv i p) ** fp) (fun x -> (inv i p) ** fp' x)
 
 val with_invariant_g
@@ -283,29 +280,29 @@ val with_invariant_g
     (#p:slprop)
     (i:iref { not (mem_inv f_opens i) })
     ($f:unit -> stt_ghost a f_opens
-                            (p ** fp)
-                            (fun x -> p ** fp' x))
+                            (later p ** fp)
+                            (fun x -> later p ** fp' x))
 : stt_ghost a (add_inv f_opens i) ((inv i p) ** fp) (fun x -> (inv i p) ** fp' x)
 
-val distinct_invariants_have_distinct_names
-    (#p #q:slprop)
-    (i j:iref)
-    (_:squash (p =!= q))
-: stt_ghost
-    (squash (i =!= j))
-    emp_inames
-    ((inv i p) ** (inv j q))
-    (fun _ -> (inv i p) ** (inv j q))
+// val distinct_invariants_have_distinct_names
+//     (#p #q:slprop)
+//     (i j:iref)
+//     (_:squash (p =!= q))
+// : stt_ghost
+//     (squash (i =!= j))
+//     emp_inames
+//     ((inv i p) ** (inv j q))
+//     (fun _ -> (inv i p) ** (inv j q))
 
 val invariant_name_identifies_invariant
       (p q:slprop)
       (i:iref)
       (j:iref { i == j })
 : stt_ghost
-    (squash (p == q))
+    unit
     emp_inames
-    ((inv i p) ** (inv j q))
-    (fun _ -> (inv i p) ** (inv j q))
+    (inv i p ** inv j q)
+    (fun _ -> inv i p ** inv j q ** InstantiatedSemantics.equiv p q)
 
 ////////////////////////////////////////////////////////////////////////
 // References
